update TCB

veric/tcb.v
@@ -1,15 +1,18 @@
 Require Import VST.sepcomp.extspec.
 Require Import VST.sepcomp.step_lemmas.
 Require Import VST.veric.base.
+Require Import VST.veric.Clight_language.
 Require Import VST.veric.juicy_extspec.
 Require Import VST.veric.juicy_mem.
+Require Import VST.veric.mpred.
+Require Import VST.veric.external_state.
 Require Import VST.veric.compspecs.
 Require Import VST.veric.semax_prog.
-Require Import VST.veric.SequentialClight2.
+Require Import VST.veric.SequentialClight.
 Require Import VST.veric.NullExtension.
 
-Definition null_extension_juicyspec : external_specification juicy_mem external_function unit
-  := Build_external_specification juicy_mem external_function unit
+Definition null_extension_extspec : external_specification mem external_function unit
+  := Build_external_specification mem external_function unit
      (*ext_spec_type*)
      (fun ef => False)
      (*ext_spec_pre*)
@@ -19,32 +22,21 @@ Definition null_extension_juicyspec : external_specification juicy_mem external_
      (*ext_spec_exit*)
      (fun rv m z => True).
 
-(* If an inline external call can run on a memory m, then it should produce the same return value
-   and perform the same memory operations when run on a memory m1 that has more permissions than m
-   but is otherwise identical. c.f. Events.ec_mem_extends *)
-Definition ec_mem_sub := forall ef se lv m t v m' (EFI : ef_inline ef = true) m1
-  (EFC : Events.external_call ef se lv m t v m'), mem_sub m m1 ->
-  exists m1' (EFC1 : Events.external_call ef se lv m1 t v m1'),
-    mem_sub m' m1' /\ proj1_sig (Clight_core.inline_external_call_mem_events _ _ _ _ _ _ _ EFI EFC1) =
-    proj1_sig (Clight_core.inline_external_call_mem_events _ _ _ _ _ _ _ EFI EFC).
-
 Theorem VST_sound: 
   {Espec : OracleKind 
-  | JMeq.JMeq (JE_spec _ (@OK_spec Espec)) null_extension_juicyspec /\
-  let dryspec :=  juicy_dry_ext_spec_make _ null_extension_juicyspec in 
-  forall (CS: compspecs)
-     (Jsub: ec_mem_sub)
+  | JMeq.JMeq (@OK_spec Espec) null_extension_extspec /\
+  forall (CS: compspecs) `(!VSTGpreS OK_ty Σ)
      (prog: Clight.program) (initial_oracle: OK_ty)
      (V : mpred.varspecs) (G : mpred.funspecs) (m: mem),
-     @semax_prog Espec CS prog initial_oracle V G ->
+     (forall {HH : heapGS Σ} {HE : externalGS OK_ty Σ}, @semax_prog _ HH Espec HE CS prog initial_oracle V G) ->
      Genv.init_mem prog = Some m ->
      exists b, exists q, exists m',
        Genv.find_symbol (Genv.globalenv prog) (prog_main prog) = Some b /\
        semantics.initial_core  (Clight_core.cl_core_sem (Clight.globalenv prog))
            0 m q m' (Vptr b Ptrofs.zero) nil /\
        forall n,
-        @dry_safeN _ _ _ unit (semax.genv_symb_injective)
-          (Clight_core.cl_core_sem (Clight.globalenv prog)) dryspec
+        @dry_safeN _ _ _ unit (genv_symb_injective)
+          (Clight_core.cl_core_sem (Clight.globalenv prog)) null_extension_extspec
            (Clight.genv_genv 
             (Clight.Build_genv (Genv.globalenv prog) (Ctypes.prog_comp_env prog)) )
              n tt q m'}.
